examples/logic/ltl/concrltl2waaScript.sml
@@ -66,78 +66,39 @@ val trans_concr_def = Define`
        (<| pos := [] ; neg := [] ; sucs := [U f1 f2] |> ::
                                            (trans_concr aP f1)))`;
 
-val expandAuto_def = Define`
-   (* (expandAuto φ = *)
-   (*    let initForms = tempDNF_concr φ *)
-   (*    in let a0 = concrAA empty [] (props_concr φ) *)
-   (*    in let a1 = FOLDL (\a s. addFrmlToAut a s) a0 (FLAT initForms) *)
-   (*    in let init_concr = *)
-   (*             MAP *)
-   (*                 (λ l. *)
-   (*                    MAP (\s. THE (findNode (λ(_,l). l.frml = s) a1.graph)) l) *)
-   (*                 initForms *)
-   (*    in let a_init = a1 with <| init := init_concr |> *)
-   (*    in expandAuto_step (FLAT initForms) a_init) *)
- (expandAuto_step [] aut = aut)
- ∧ (expandAuto_step (f::fs) (concrAA g init aP) =
-     let a1 = addFrmlToAut (concrAA g init aP) f
-     in let trans = trans_concr aP f
-     in let allSucs = FOLDL (\pr e. e.sucs ++ pr) [] trans
-     in let a2 = FOLDL (\g p. addFrmlToAut g p) a1 allSucs
-     in let a3 = FOLDL (\a e. addEdgeToAut f e a) a2 trans
-     in let restNodes = FILTER (\s. ~ (inAuto (concrAA g init aP) s)) allSucs
-     in expandAuto_step (restNodes++fs) a3)`;
-  (qexists_tac `λ(ls,a) (ls2,a2).
-          NoNodeProcessedTwice (HD ls) (a,ls) (a2,ls2)`
-   >> rpt strip_tac
-    >- (`!g. WF (NoNodeProcessedTwice g)` suffices_by (
-           qabbrev_tac `f = 
-)
+val tempSubfCl_def = Define`
+  tempSubfCl l = BIGUNION { tempSubForms f | MEM f l }`;
 
-[NNPT_WF])
- )
-
-;
 
 val NoNodeProcessedTwice_def = Define`
   NoNodeProcessedTwice g (a,ns) (a2,ns2) =
-    ((tempSubForms g DIFF {x | inAuto a x }
-                  ⊂ tempSubForms g DIFF {x | inAuto a2 x })
-         \/ ((tempSubForms g DIFF {x | inAuto a x }
-              = tempSubForms g DIFF {x | inAuto a2 x })
-              ∧ ((list_size (\x. 1) ns)
-                  < (list_size (\x. 1) ns2))))`;
+    ((g DIFF (LIST_TO_SET (autoStates a))
+                  ⊂ g DIFF (LIST_TO_SET (autoStates a2)))
+         \/ ((g DIFF (LIST_TO_SET (autoStates a))
+              = g DIFF (LIST_TO_SET (autoStates a2)))
+              ∧ (LENGTH ns) < (LENGTH ns2)))`;
 
 val NNPT_WF = store_thm
  ("NNPT_WF",
-  ``!g. WF (NoNodeProcessedTwice g)``,
+  ``!g. FINITE g ==> WF (NoNodeProcessedTwice g)``,
    rpt strip_tac
-   >> `WF (λ(s:α ltl_frml -> bool) t. s ⊂ t
-         ∧ s ⊆ tempSubForms g
-         ∧ t ⊆ tempSubForms g)` by (
-       `FINITE (tempSubForms g)` by metis_tac[TSF_FINITE]
-       >> metis_tac[PSUBSET_WF]
-   )
+   >> `WF (λs t. s ⊂ t
+         ∧ s ⊆ g ∧ t ⊆ g)` by metis_tac[PSUBSET_WF]
    >> `WF ($<)` by metis_tac[WF_LESS]
-   >> `WF (λ(x:num list) y.
-            list_size (\n. n) x < list_size (\n. n) y)` by (
-       qabbrev_tac `f = \x:num list. list_size (\n. n) x`
-       >> `inv_image ($<) f =
-            (λx:num list y.
-              list_size (λn. n) x < list_size (λn. n) y)` by (
-           simp[inv_image_def]
-       )
-       >> `WF (inv_image ($<) f)` suffices_by fs[]
+   >> `WF (λ (x:β list) (y:β list).
+            LENGTH x < LENGTH y)` by (
+       `inv_image ($<) LENGTH
+              = (λ(x:β list) (y:β list).
+                  LENGTH x < LENGTH y)` by simp[inv_image_def]
+       >> `WF (inv_image ($<) (LENGTH:(β list -> num)))` suffices_by fs[]
        >> metis_tac[WF_inv_image]
    )
-   >> qabbrev_tac `P = (λs t. s ⊂ t ∧ s ⊆ tempSubForms g ∧ t ⊆ tempSubForms g)`
-   >> qabbrev_tac
-         `Q = (λ x y.
-                list_size (λn. n) x < list_size (λn. n) y)`
-   >> qabbrev_tac `f = λ a. tempSubForms g DIFF {x | inAuto a x }`
+   >> qabbrev_tac `P = (λs t. s ⊂ t ∧ s ⊆ g ∧ t ⊆ g)`
+   >> qabbrev_tac `Q = (λ(x:β list) (y:β list). LENGTH x < LENGTH y)`
+   >> qabbrev_tac `f = λ a. g DIFF (LIST_TO_SET (autoStates a))`
    >> `inv_image P f = λ a a2.
-                        (tempSubForms g DIFF {x | inAuto a x }
-                         ⊂ tempSubForms g DIFF {x | inAuto a2 x })` by (
+                        (g DIFF (LIST_TO_SET (autoStates a))
+                         ⊂ g DIFF (LIST_TO_SET (autoStates a2)))` by (
       qunabbrev_tac `P`
       >> fs[inv_image_def]
       >> `(\x y. f x ⊂ f y) = (λa a2. f a ⊂ f a2)`
@@ -149,7 +110,7 @@ val NNPT_WF = store_thm
    >> `WF (inv_image P f)` by metis_tac[WF_inv_image]
    >> `WF (P LEX Q)` by metis_tac[WF_LEX]
    >> qabbrev_tac
-        `j = λ(a,l:num list). (tempSubForms g DIFF {x | inAuto a x},l)`
+        `j = λ(a,(l:β list)). (g DIFF (LIST_TO_SET (autoStates a)),l)`
    >> `WF (inv_image (P LEX Q) j)` by metis_tac[WF_inv_image]
    >> `!x y. (NoNodeProcessedTwice g) x y ==> (inv_image (P LEX Q) j) x y` by (
        fs[inv_image_def,LEX_DEF] >> rpt strip_tac
@@ -161,12 +122,116 @@ val NNPT_WF = store_thm
    >> metis_tac[WF_SUBSET]
  );
 
-
-
-
-
-(* val concrLtl2Waa_def = Define` *)
-
+(* val expandAuto_def = Define` *)
+(*    (* (expandAuto φ = *) *)
+(*    (*    let initForms = tempDNF_concr φ *) *)
+(*    (*    in let a0 = concrAA empty [] (props_concr φ) *) *)
+(*    (*    in let a1 = FOLDL (\a s. addFrmlToAut a s) a0 (FLAT initForms) *) *)
+(*    (*    in let init_concr = *) *)
+(*    (*             MAP *) *)
+(*    (*                 (λ l. *) *)
+(*    (*                    MAP (\s. THE (findNode (λ(_,l). l.frml = s) a1.graph)) l) *) *)
+(*    (*                 initForms *) *)
+(*    (*    in let a_init = a1 with <| init := init_concr |> *) *)
+(*    (*    in expandAuto_step (FLAT initForms) a_init) *) *)
+(*  (expandAuto_step aut [] = SOME aut) *)
+(*  ∧ (expandAuto_step (concrAA g init aP) (f::fs)  = *)
+(*     if wfg g *)
+(*     then *)
+(*      let a1 = addFrmlToAut (concrAA g init aP) f *)
+(*      in let trans = trans_concr aP f *)
+(*      in let allSucs = FOLDR (\e pr. e.sucs ++ pr) [] trans *)
+(*      in let a2 = FOLDR (\p g. addFrmlToAut g p) a1 allSucs *)
+(*      in let a3 = *)
+(*             FOLDR (\e a_opt. case a_opt of *)
+(*                            | NONE => NONE *)
+(*                            | SOME a => addEdgeToAut f e a) *)
+(*                   (SOME a2) trans *)
+(*      in let restNodes = FILTER (\s. ~(inAuto (concrAA g init aP) s)) allSucs *)
+(*      in case a3 of *)
+(*          | NONE => NONE *)
+(*          | SOME aut => expandAuto_step aut (restNodes++fs) *)
+(*     else NONE )`; *)
+(*   (WF_REL_TAC `λ(a,ls) (a2,ls2). *)
+(*                (tempSubfCl ((autoStates a) ++ ls) *)
+(*                 = tempSubfCl ((autoStates a2) ++ ls2)) *)
+(*           ∧ NoNodeProcessedTwice *)
+(*                (tempSubfCl ((autoStates a) ++ls)) *)
+(*                (a,ls) *)
+(*                (a2,ls2)` *)
+(*     >- (qabbrev_tac *)
+(*          `b:(α concrAA # (α ltl_frml) list *)
+(*              -> (α ltl_frml -> bool)) *)
+(*                     = λ(a,l). tempSubfCl ((autoStates a) ++ l)` *)
+(*         >> qabbrev_tac *)
+(*             `P = NoNodeProcessedTwice:((α ltl_frml -> bool) *)
+(*                                        -> α concrAA # (α ltl_frml) list *)
+(*                                        -> α concrAA # (α ltl_frml) list *)
+(*                                        -> bool)` *)
+(*         >> `!(a l:(α ltl_frml) list) . FINITE (b (a,l))` by ( *)
+(*              rpt strip_tac >> qunabbrev_tac `b` *)
+(*              >> rw[tempSubfCl_def] *)
+(*               >-( `FINITE (IMAGE tempSubForms *)
+(*                                {f | MEM f (autoStates a) ∨ MEM f l })` *)
+(*                      suffices_by simp[IMAGE_DEF] *)
+(*                >> `FINITE {f | MEM f (autoStates a) ∨ MEM f l}` suffices_by *)
+(*                     metis_tac[IMAGE_FINITE] *)
+(*                >> `{f | MEM f (autoStates a) ∨ MEM f l} *)
+(*                      = LIST_TO_SET (autoStates a) ∪ (LIST_TO_SET l)` by ( *)
+(*                    simp[SET_EQ_SUBSET,SUBSET_DEF] >> rpt strip_tac *)
+(*                     ) *)
+(*                >> `(FINITE (set (autoStates a))) ∧ (FINITE (set l))` *)
+(*                     suffices_by  metis_tac[FINITE_UNION] *)
+(*                >> rpt strip_tac >> metis_tac[FINITE_LIST_TO_SET]) *)
+(*               >- metis_tac[TSF_FINITE] *)
+(*               >- metis_tac[TSF_FINITE] *)
+(*          ) *)
+(*         >> `∀g. FINITE g ⇒ WF (P g)` by metis_tac[NNPT_WF] *)
+(*         >> imp_res_tac WF_LEMM *)
+(*         >> first_x_assum (qspec_then `b` mp_tac) >> simp[] >> rpt strip_tac *)
+(*         >> `∀k. FINITE (b k)` by (rpt strip_tac >> Cases_on `k` >> fs[]) *)
+(*         >> fs[LAMBDA_PROD] >> qunabbrev_tac `P` >> qunabbrev_tac `b` *)
+(*         >> fs[] *)
+(*        ) *)
+(*     >- (rpt strip_tac >> fs[] *)
+(*      >- (simp[tempSubfCl_def,BIGUNION,SET_EQ_SUBSET] >> rpt strip_tac *)
+(*       >- (fs[inAuto_def,SUBSET_DEF] >> rpt strip_tac *)
+(*        >- (qexists_tac `s` >> fs[] >> rename[`MEM f_new _`] *)
+(*            >> qexists_tac `f_new` >> fs[] *)
+(*            >> `MEM f_new (autoStates (concrAA g init aP))` suffices_by fs[] *)
+(*            >> `set (autoStates (concrAA g init aP)) *)
+(*                 ⊆ set (autoStates (FOLDR (λp g. addFrmlToAut g p) *)
+(*                    (addFrmlToAut (concrAA g init aP) f) *)
+(*                    (FOLDR (λe pr. e.sucs ++ pr) [] (trans_concr aP f))))` by ( *)
+(*               `set (autoStates (concrAA g init aP)) *)
+(*                 ⊆ set (autoStates (addFrmlToAut (concrAA g init aP) f)) *)
+(*                        ∧ wfg (addFrmlToAut (concrAA g init aP) f).graph` by ( *)
+(*                   `(concrAA g init aP).graph = g` by fs[] *)
+(*                   >> metis_tac[ADDFRML_LEMM]) *)
+(*               >> metis_tac[ADDFRML_FOLDR_LEMM,SUBSET_TRANS] *)
+(*             ) *)
+(*            >> `set *)
+(*                 (autoStates *)
+(*                      (FOLDR (λp g. addFrmlToAut g p) *)
+(*                         (addFrmlToAut (concrAA g init aP) f) *)
+(*                         (FOLDR (λe pr. e.sucs ++ pr) [] (trans_concr aP f)))) *)
+(*               = set (autoStates aut)` by ( *)
+(*                 Induct_on `trans_concr aP f` >> rpt strip_tac >> fs[] *)
+(*                 >- (`trans_concr aP f = []` by simp[] >> fs[]) *)
+(*                 >- (`trans_concr aP f = h::v` by simp[] >> fs[] >> rw[] *)
+(*                     >> Cases_on ` *)
+(*                          FOLDR *)
+(*                         (λe a_opt. *)
+(*                          case a_opt of *)
+(*                              NONE => NONE *)
+(*                            | SOME a => addEdgeToAut f e a) *)
+(*                         (SOME *)
+(*                          (FOLDR (λp g. addFrmlToAut g p) *)
+(*                                 (addFrmlToAut (concrAA g init aP) f) *)
+(*                                 (h.sucs ++ FOLDR (λe pr. e.sucs ++ pr) [] v) *)
+(*                         )) v` >> fs[] *)
+                    
+(* ) *)
 
 
 
